heap_lang/lifting.v
@@ -9,13 +9,17 @@ Section lifting.
 Context {Σ : iFunctor}.
 Implicit Types P Q : iProp heap_lang Σ.
 Implicit Types Φ : val → iProp heap_lang Σ.
-Implicit Types K : ectx.
 Implicit Types ef : option (expr []).
 
 (** Bind. This bundles some arguments that wp_ectx_bind leaves as indices. *)
 Lemma wp_bind {E e} K Φ :
   WP e @ E {{ λ v, WP fill K (of_val v) @ E {{ Φ }} }} ⊢ WP fill K e @ E {{ Φ }}.
 Proof. exact: wp_ectx_bind. Qed.
+
+Lemma wp_bindi {E e} Ki Φ :
+  WP e @ E {{ λ v, WP fill_item Ki (of_val v) @ E {{ Φ }} }} ⊢
+     WP fill_item Ki e @ E {{ Φ }}.
+Proof. exact: weakestpre.wp_bind. Qed.
 
 (** Base axioms for core primitives of the language: Stateful reductions. *)
 Lemma wp_alloc_pst E σ e v Φ :
