program_logic/ectxi_language.v
@@ -1,0 +1,111 @@
+(** An axiomatization of languages based on evaluation context items, including
+    a proof that these are instances of general ectx-based languages. *)
+From iris.algebra Require Export base.
+From iris.program_logic Require Import language ectx_language.
+
+(* We need to make thos arguments indices that we want canonical structure
+   inference to use a keys. *)
+Class EctxiLanguage (expr val ectx_item state : Type) := {
+  of_val : val → expr;
+  to_val : expr → option val;
+  fill_item : ectx_item → expr → expr;
+  atomic : expr → Prop;
+  head_step : expr → state → expr → state → option expr → Prop;
+
+  to_of_val v : to_val (of_val v) = Some v;
+  of_to_val e v : to_val e = Some v → of_val v = e;
+  val_stuck e1 σ1 e2 σ2 ef : head_step e1 σ1 e2 σ2 ef → to_val e1 = None;
+
+  fill_item_inj Ki :> Inj (=) (=) (fill_item Ki);
+  fill_item_val Ki e : is_Some (to_val (fill_item Ki e)) → is_Some (to_val e);
+  fill_item_no_val_inj Ki1 Ki2 e1 e2 :
+    to_val e1 = None → to_val e2 = None →
+    fill_item Ki1 e1 = fill_item Ki2 e2 → Ki1 = Ki2;
+
+  head_ctx_step_val Ki e σ1 e2 σ2 ef :
+    head_step (fill_item Ki e) σ1 e2 σ2 ef → is_Some (to_val e);
+
+  atomic_not_val e : atomic e → to_val e = None;
+  atomic_step e1 σ1 e2 σ2 ef :
+    atomic e1 →
+    head_step e1 σ1 e2 σ2 ef →
+    is_Some (to_val e2);
+  atomic_fill_item e Ki :
+    atomic (fill_item Ki e) → is_Some (to_val e)
+}.
+
+Arguments of_val {_ _ _ _ _} _.
+Arguments to_val {_ _ _ _ _} _.
+Arguments fill_item {_ _ _ _ _} _ _.
+Arguments atomic {_ _ _ _ _} _.
+Arguments head_step {_ _ _ _ _} _ _ _ _ _.
+
+Arguments to_of_val {_ _ _ _ _} _.
+Arguments of_to_val {_ _ _ _ _} _ _ _.
+Arguments val_stuck {_ _ _ _ _} _ _ _ _ _ _.
+Arguments fill_item_val {_ _ _ _ _} _ _ _.
+Arguments fill_item_no_val_inj {_ _ _ _ _} _ _ _ _ _ _ _.
+Arguments head_ctx_step_val {_ _ _ _ _} _ _ _ _ _ _ _.
+Arguments step_by_val {_ _ _ _ _} _ _ _ _ _ _ _ _ _ _ _.
+Arguments atomic_not_val {_ _ _ _ _} _ _.
+Arguments atomic_step {_ _ _ _ _} _ _ _ _ _ _ _.
+Arguments atomic_fill_item {_ _ _ _ _} _ _ _.
+
+Section ectxi_language.
+  Context {expr val ectx_item state}
+          {Λ : EctxiLanguage expr val ectx_item state}.
+  Implicit Types (e : expr) (Ki : ectx_item).
+  Notation ectx := (list ectx_item).
+
+  Definition fill (K : ectx) (e : expr) : expr := fold_right fill_item e K.
+
+  Instance fill_inj K : Inj (=) (=) (fill K).
+  Proof. red; induction K as [|Ki K IH]; naive_solver. Qed.
+
+  Lemma fill_val K e : is_Some (to_val (fill K e)) → is_Some (to_val e).
+  Proof.
+    induction K; simpl; first done. intros ?%fill_item_val. eauto.
+  Qed.
+
+  Lemma fill_not_val K e : to_val e = None → to_val (fill K e) = None.
+  Proof. rewrite !eq_None_not_Some. eauto using fill_val. Qed.
+
+  Lemma atomic_fill K e : atomic (fill K e) → to_val e = None → K = [].
+  Proof.
+    destruct K as [|Ki K]; [done|].
+    rewrite eq_None_not_Some=> /= ? []; eauto using atomic_fill_item, fill_val.
+  Qed.
+
+  (* When something does a step, and another decomposition of the same expression
+  has a non-val [e] in the hole, then [K] is a left sub-context of [K'] - in
+  other words, [e] also contains the reducible expression *)
+  Lemma step_by_val K K' e1 e1' σ1 e2 σ2 ef :
+    fill K e1 = fill K' e1' → to_val e1 = None → head_step e1' σ1 e2 σ2 ef →
+    exists K'', K' = K ++ K''. (* K `prefix_of` K' *)
+  Proof.
+    intros Hfill Hred Hnval; revert K' Hfill.
+    induction K as [|Ki K IH]; simpl; intros K' Hfill; first by eauto.
+    destruct K' as [|Ki' K']; simplify_eq/=.
+    { exfalso; apply (eq_None_not_Some (to_val (fill K e1)));
+      eauto using fill_not_val, head_ctx_step_val. }
+    cut (Ki = Ki'); [naive_solver eauto using prefix_of_cons|].
+    eauto using fill_item_no_val_inj, val_stuck, fill_not_val.
+  Qed.
+
+  Global Program Instance : EctxLanguage expr val ectx state :=
+    (* For some reason, Coq always rejects the record syntax claiming I
+       fixed fields of different records, even when I did not. *)
+    Build_EctxLanguage expr val ectx state of_val to_val [] (++) fill atomic head_step _ _ _ _ _ _ _ _ _ _ _ _.
+  Solve Obligations with eauto using to_of_val, of_to_val, val_stuck,
+    atomic_not_val, atomic_step, fill_not_val, atomic_fill,
+    step_by_val, fold_right_app, app_eq_nil.
+
+  Global Instance ectxi_lang_ctx_item Ki :
+    LanguageCtx (ectx_lang expr) (fill_item Ki).
+  Proof. change (LanguageCtx _ (fill [Ki])). apply _. Qed.
+
+End ectxi_language.
+
+
+
+
